Foundation/Modal/Kripke/Hilbert/Grz/Completeness.lean
@@ -41,15 +41,10 @@ lemma mem_left (h : ψ ∈ φ.subformulas) : ψ ∈ φ.subformulasGrz := by
   left;
   tauto;
 
-
-
 end subformulasGrz
 
 end Formula
 
-
-
-namespace Hilbert.Grz.Kripke
 
 open Formula
 open Formula.Kripke
@@ -58,23 +53,28 @@ open Entailment.Context
 open ComplementClosedConsistentFinset
 open Kripke
 
+namespace Kripke.Grz
+
+variable {S} [Entailment (Formula ℕ) S]
+variable {𝓢 : S} [Entailment.Consistent 𝓢] [Entailment.Grz 𝓢]
+
 variable {φ ψ : Formula ℕ}
 
-abbrev miniCanonicalFrame (φ : Formula ℕ) : Kripke.Frame where
-  World := ComplementClosedConsistentFinset (Hilbert.Grz) (φ.subformulasGrz)
+abbrev miniCanonicalFrame (𝓢 : S) [Entailment.Grz 𝓢] [Entailment.Consistent 𝓢] (φ : Formula ℕ) : Kripke.Frame where
+  World := ComplementClosedConsistentFinset 𝓢 (φ.subformulasGrz)
   Rel X Y :=
     (∀ ψ ∈ □''⁻¹(φ.subformulasGrz), □ψ ∈ X → □ψ ∈ Y) ∧
     ((∀ ψ ∈ □''⁻¹(φ.subformulasGrz), □ψ ∈ Y → □ψ ∈ X) → X = Y)
 
 namespace miniCanonicalFrame
 
-instance : (miniCanonicalFrame φ).IsFinite := by
+instance : (miniCanonicalFrame 𝓢 φ).IsFinite := by
   apply Kripke.Frame.isFinite_iff _ |>.mpr;
   infer_instance;
 
-lemma reflexive : Reflexive (miniCanonicalFrame φ).Rel := by simp [Reflexive];
+lemma reflexive : Reflexive (miniCanonicalFrame 𝓢 φ).Rel := by simp [Reflexive];
 
-lemma transitive : Transitive (miniCanonicalFrame φ).Rel := by
+lemma transitive : Transitive (miniCanonicalFrame 𝓢 φ).Rel := by
   simp only [Transitive];
   rintro X Y Z ⟨RXY₁, RXY₂⟩ ⟨RYZ₁, RYZ₂⟩;
   constructor;
@@ -90,20 +90,20 @@ lemma transitive : Transitive (miniCanonicalFrame φ).Rel := by
     subst_vars;
     tauto;
 
-lemma antisymm : AntiSymmetric (miniCanonicalFrame φ).Rel := by
+lemma antisymm : AntiSymmetric (miniCanonicalFrame 𝓢 φ).Rel := by
   rintro X Y ⟨_, h₁⟩ ⟨h₂, _⟩;
   exact h₁ h₂;
 
 end miniCanonicalFrame
 
 
-abbrev miniCanonicalModel (φ : Formula ℕ) : Kripke.Model where
-  toFrame := miniCanonicalFrame φ
+abbrev miniCanonicalModel (𝓢 : S) [Entailment.Grz 𝓢] [Entailment.Consistent 𝓢] (φ : Formula ℕ) : Kripke.Model where
+  toFrame := miniCanonicalFrame 𝓢 φ
   Val X a := (atom a) ∈ X
 
-
+omit [Consistent 𝓢] [Entailment.Grz 𝓢] in
 lemma truthlemma_lemma1
-  {X : ComplementClosedConsistentFinset (Hilbert.Grz) (φ.subformulasGrz)} (hq : □ψ ∈ φ.subformulas)
+  {X : ComplementClosedConsistentFinset 𝓢 (φ.subformulasGrz)} (hq : □ψ ∈ φ.subformulas)
   : ((X.1.prebox.box) ∪ {□(ψ ➝ □ψ), -ψ}) ⊆ (φ.subformulasGrz)⁻ := by
   simp only [FormulaFinset.complementary];
   intro χ hr;
@@ -125,9 +125,10 @@ lemma truthlemma_lemma1
       exact subformulas.mem_box hq;
     . rfl;
 
+omit [Consistent 𝓢] in
 lemma truthlemma_lemma2
-  {X : ComplementClosedConsistentFinset (Hilbert.Grz) (φ.subformulasGrz)} (hq₁ : □ψ ∈ φ.subformulas) (hq₂ : □ψ ∉ X)
-  : FormulaFinset.Consistent (Hilbert.Grz) ((X.1.prebox.box) ∪ {□(ψ ➝ □ψ), -ψ}) := by
+  {X : ComplementClosedConsistentFinset 𝓢 (φ.subformulasGrz)} (hq₁ : □ψ ∈ φ.subformulas) (hq₂ : □ψ ∉ X)
+  : FormulaFinset.Consistent 𝓢 ((X.1.prebox.box) ∪ {□(ψ ➝ □ψ), -ψ}) := by
     apply FormulaFinset.intro_union_consistent;
     rintro Γ₁ Γ₂ ⟨hΓ₁, hΓ₂⟩;
     replace hΓ₂ : ∀ χ ∈ Γ₂, χ = □(ψ ➝ □ψ) ∨ χ = -ψ := by
@@ -135,32 +136,32 @@ lemma truthlemma_lemma2
       simpa using hΓ₂ χ hr;
 
     by_contra hC;
-    have : Γ₁ ⊢[(Hilbert.Grz)]! ⋀Γ₂ ➝ ⊥ := and_imply_iff_imply_imply'!.mp hC;
-    have : Γ₁ ⊢[(Hilbert.Grz)]! (□(ψ ➝ □ψ) ⋏ -ψ) ➝ ⊥ := imp_trans''! (by
-      suffices Γ₁ ⊢[(Hilbert.Grz)]! ⋀[□(ψ ➝ □ψ), -ψ] ➝ ⋀Γ₂ by
+    have : Γ₁ ⊢[𝓢]! ⋀Γ₂ ➝ ⊥ := and_imply_iff_imply_imply'!.mp hC;
+    have : Γ₁ ⊢[𝓢]! (□(ψ ➝ □ψ) ⋏ -ψ) ➝ ⊥ := imp_trans''! (by
+      suffices Γ₁ ⊢[𝓢]! ⋀[□(ψ ➝ □ψ), -ψ] ➝ ⋀Γ₂ by
         simpa only [ne_eq, List.cons_ne_self, not_false_eq_true, List.conj₂_cons_nonempty, List.conj₂_singleton];
       apply conjconj_subset!;
       simpa using hΓ₂;
     ) this;
-    have : Γ₁ ⊢[(Hilbert.Grz)]! □(ψ ➝ □ψ) ➝ -ψ ➝ ⊥ := and_imply_iff_imply_imply'!.mp this;
-    have : Γ₁ ⊢[(Hilbert.Grz)]! □(ψ ➝ □ψ) ➝ ψ := by
+    have : Γ₁ ⊢[𝓢]! □(ψ ➝ □ψ) ➝ -ψ ➝ ⊥ := and_imply_iff_imply_imply'!.mp this;
+    have : Γ₁ ⊢[𝓢]! □(ψ ➝ □ψ) ➝ ψ := by
       rcases Formula.complement.or (φ := ψ) with (hp | ⟨ψ, rfl⟩);
       . rw [hp] at this;
         exact imp_trans''! this dne!;
       . simpa only [complement] using this;
-    have : (□'Γ₁) ⊢[(Hilbert.Grz)]! □(□(ψ ➝ □ψ) ➝ ψ) := contextual_nec! this;
-    have : (□'Γ₁) ⊢[(Hilbert.Grz)]! ψ := axiomGrz! ⨀ this;
-    have : (Hilbert.Grz) ⊢! ⋀□'□'Γ₁ ➝ □ψ := contextual_nec! this;
-    have : (Hilbert.Grz) ⊢! □□⋀Γ₁ ➝ □ψ := imp_trans''! (imp_trans''! (distribute_multibox_conj! (n := 2)) $ conjconj_subset! (λ _ => List.mem_multibox_add.mp)) this;
-    have : (Hilbert.Grz) ⊢! □⋀Γ₁ ➝ □ψ := imp_trans''! axiomFour! this;
-    have : (Hilbert.Grz) ⊢! ⋀□'Γ₁ ➝ □ψ := imp_trans''! collect_box_conj! this;
-    have : (Hilbert.Grz) ⊢! ⋀□'(X.1.prebox.box |>.toList) ➝ □ψ := imp_trans''! (conjconj_subset! (by
+    have : (□'Γ₁) ⊢[𝓢]! □(□(ψ ➝ □ψ) ➝ ψ) := contextual_nec! this;
+    have : (□'Γ₁) ⊢[𝓢]! ψ := axiomGrz! ⨀ this;
+    have : 𝓢 ⊢! ⋀□'□'Γ₁ ➝ □ψ := contextual_nec! this;
+    have : 𝓢 ⊢! □□⋀Γ₁ ➝ □ψ := imp_trans''! (imp_trans''! (distribute_multibox_conj! (n := 2)) $ conjconj_subset! (λ _ => List.mem_multibox_add.mp)) this;
+    have : 𝓢 ⊢! □⋀Γ₁ ➝ □ψ := imp_trans''! axiomFour! this;
+    have : 𝓢 ⊢! ⋀□'Γ₁ ➝ □ψ := imp_trans''! collect_box_conj! this;
+    have : 𝓢 ⊢! ⋀□'(X.1.prebox.box |>.toList) ➝ □ψ := imp_trans''! (conjconj_subset! (by
       intro ξ hξ;
       obtain ⟨χ, hχ, rfl⟩ := List.exists_of_box hξ;
       apply List.box_mem_of;
       simpa using hΓ₁ χ hχ;
     )) this;
-    have : (Hilbert.Grz) ⊢! ⋀□'(X.1.prebox.toList) ➝ □ψ := imp_trans''! (conjconj_provable! (by
+    have : 𝓢 ⊢! ⋀□'(X.1.prebox.toList) ➝ □ψ := imp_trans''! (conjconj_provable! (by
       intro ψ hψ;
       obtain ⟨ξ, hξ, rfl⟩ := List.exists_of_box hψ;
       obtain ⟨χ, hχ, rfl⟩ := by simpa using hξ;
@@ -169,7 +170,7 @@ lemma truthlemma_lemma2
       apply List.box_mem_of;
       simpa;
     )) this;
-    have : X *⊢[(Hilbert.Grz)]! □ψ := by
+    have : X *⊢[𝓢]! □ψ := by
       apply Context.provable_iff.mpr;
       use □'X.1.prebox.toList;
       constructor;
@@ -180,21 +181,14 @@ lemma truthlemma_lemma2
     have : □ψ ∈ X := membership_iff (by trivial) |>.mpr this;
     contradiction;
 
--- TODO: syntactical proof
-lemma truthlemma_lemma3 : (Hilbert.Grz) ⊢! (φ ⋏ □(φ ➝ □φ)) ➝ □φ := by
-  apply KT_weakerThan_Grz.pbl;
-  by_contra hC;
-  have := (not_imp_not.mpr $ Hilbert.KT.Kripke.complete |>.complete) hC;
-  simp at this;
-  obtain ⟨F, F_refl, hF⟩ := Kripke.exists_frame_of_not_validOnFrameClass this;
-  simp [ValidOnFrame, ValidOnModel, Satisfies, Semantics.Realize] at hF;
-  obtain ⟨V, x, h₁, h₂, ⟨y, Rxy, h₃⟩⟩ := hF;
-  have := h₂ x (F_refl x);
-  have := (this h₁) _ Rxy;
-  contradiction;
+omit [Consistent 𝓢] in
+lemma truthlemma_lemma3 : 𝓢 ⊢! (φ ⋏ □(φ ➝ □φ)) ➝ □φ := by
+  refine imp_trans''! ?_ $ mdp_in! (𝓢 := 𝓢) (φ := φ) (ψ := □φ);
+  apply and_replace_right!;
+  exact axiomT!;
 
-lemma truthlemma {X : (miniCanonicalModel φ).World} (q_sub : ψ ∈ φ.subformulas) :
-  Satisfies (miniCanonicalModel φ) X ψ ↔ ψ ∈ X := by
+lemma truthlemma {X : (miniCanonicalModel 𝓢 φ).World} (q_sub : ψ ∈ φ.subformulas) :
+  Satisfies (miniCanonicalModel 𝓢 φ) X ψ ↔ ψ ∈ X := by
   induction ψ using Formula.rec' generalizing X with
   | hatom => simp [Satisfies];
   | hfalsum => simp [Satisfies];
@@ -240,7 +234,7 @@ lemma truthlemma {X : (miniCanonicalModel φ).World} (q_sub : ψ ∈ φ.subformu
     . contrapose;
       by_cases w : ψ ∈ X;
       . intro h;
-        obtain ⟨Y, hY⟩ := lindenbaum (𝓢 := Hilbert.Grz) (Ψ := φ.subformulasGrz) (truthlemma_lemma1 q_sub) (truthlemma_lemma2 q_sub h);
+        obtain ⟨Y, hY⟩ := lindenbaum (𝓢 := 𝓢) (truthlemma_lemma1 q_sub) (truthlemma_lemma2 q_sub h);
         simp only [Finset.union_subset_iff] at hY;
         simp only [Satisfies]; push_neg;
         use Y;
@@ -254,12 +248,13 @@ lemma truthlemma {X : (miniCanonicalModel φ).World} (q_sub : ψ ∈ φ.subformu
             use (ψ ➝ □ψ);
             refine ⟨?_, ?_, ?_⟩;
             . simp_all;
-            . apply hY.2; simp;
+            . apply hY.2;
+              simp;
             . by_contra hC;
-              have : ↑X *⊢[Hilbert.Grz]! ψ := membership_iff (subformulasGrz.mem_left (by assumption)) |>.mp w;
-              have : ↑X *⊢[(Hilbert.Grz)]! □(ψ ➝ □ψ) := membership_iff (by simp; right; assumption) |>.mp hC;
-              have : ↑X *⊢[(Hilbert.Grz)]! (ψ ⋏ □(ψ ➝ □ψ)) ➝ □ψ := Context.of! $ truthlemma_lemma3;
-              have : ↑X *⊢[(Hilbert.Grz)]! □ψ := this ⨀ and₃'! (by assumption) (by assumption);
+              have : ↑X *⊢[𝓢]! ψ := membership_iff (subformulasGrz.mem_left (by assumption)) |>.mp w;
+              have : ↑X *⊢[𝓢]! □(ψ ➝ □ψ) := membership_iff (by simp; right; assumption) |>.mp hC;
+              have : ↑X *⊢[𝓢]! (ψ ⋏ □(ψ ➝ □ψ)) ➝ □ψ := Context.of! $ truthlemma_lemma3;
+              have : ↑X *⊢[𝓢]! □ψ := this ⨀ and₃'! (by assumption) (by assumption);
               have : □ψ ∈ X := membership_iff (subformulasGrz.mem_origin (by assumption)) |>.mpr this;
               contradiction;
         . apply ih (by aesop) |>.not.mpr;
@@ -275,37 +270,49 @@ lemma truthlemma {X : (miniCanonicalModel φ).World} (q_sub : ψ ∈ φ.subformu
         . exact ih (by aesop) |>.not.mpr w;
     . intro h Y RXY;
       apply ih (subformulas.mem_box q_sub) |>.mpr;
-      have : ↑Y *⊢[(Hilbert.Grz)]! □ψ ➝ ψ := Context.of! $ axiomT!;
-      have : ↑Y *⊢[(Hilbert.Grz)]! ψ := this ⨀
+      have : ↑Y *⊢[𝓢]! □ψ ➝ ψ := Context.of! $ axiomT!;
+      have : ↑Y *⊢[𝓢]! ψ := this ⨀
         (membership_iff (by apply subformulasGrz.mem_left; assumption) |>.mp (RXY.1 ψ (by apply subformulasGrz.mem_left; tauto) h));
       exact membership_iff (by apply subformulasGrz.mem_left; exact subformulas.mem_box q_sub) |>.mpr this;
 
-instance complete : Complete (Hilbert.Grz) Kripke.FrameClass.finite_strict_preorder := ⟨by
+lemma complete_of_mem_miniCanonicalFrame
+  (C : Kripke.FrameClass)
+  (hC : ∀ {φ}, miniCanonicalFrame 𝓢 φ ∈ C)
+  : Complete 𝓢 C := ⟨by
   intro φ;
   contrapose;
   intro h;
   apply Semantics.set_models_iff.not.mpr;
   push_neg;
-  use (miniCanonicalFrame φ);
+  use (miniCanonicalFrame 𝓢 φ);
   constructor;
-  . refine ⟨inferInstance, miniCanonicalFrame.reflexive, miniCanonicalFrame.transitive, miniCanonicalFrame.antisymm⟩;
-  . apply ValidOnFrame.not_of_exists_model_world;
-    obtain ⟨X, hX₁⟩ := lindenbaum (𝓢 := Hilbert.Grz) (Φ := {-φ}) (Ψ := φ.subformulasGrz)
+  . apply hC;
+  . apply ValidOnFrame.not_of_exists_valuation_world;
+    obtain ⟨X, hX₁⟩ := lindenbaum (𝓢 := 𝓢) (Φ := {-φ}) (Ψ := φ.subformulasGrz)
       (by
         simp only [Finset.singleton_subset_iff];
         apply FormulaFinset.complementary_comp;
         exact subformulasGrz.mem_self
       )
       (FormulaFinset.unprovable_iff_singleton_compl_consistent.mpr h);
-    use (miniCanonicalModel φ), X;
-    constructor;
-    . rfl;
-    . apply truthlemma (by simp) |>.not.mpr;
-      exact iff_mem_compl (by simp) |>.not.mpr $ by
-        push_neg;
-        apply hX₁;
-        tauto;
+    use (miniCanonicalModel _ φ).Val, X;
+    apply truthlemma (by simp) |>.not.mpr;
+    exact iff_mem_compl (by simp) |>.not.mpr $ by
+      push_neg;
+      apply hX₁;
+      tauto;
 ⟩
+
+end Kripke.Grz
+
+
+namespace Hilbert.Grz.Kripke
+
+open Kripke.Grz
+
+instance complete : Complete (Hilbert.Grz) FrameClass.finite_partial_order :=
+  complete_of_mem_miniCanonicalFrame FrameClass.finite_partial_order  $ by
+    refine ⟨inferInstance, miniCanonicalFrame.reflexive, miniCanonicalFrame.transitive, miniCanonicalFrame.antisymm⟩;
 
 end Hilbert.Grz.Kripke
 
