Foundation/Modal/Kripke/Hilbert/Grz/Soundness.lean
@@ -12,22 +12,22 @@ open Hilbert.Kripke
 namespace Kripke
 
 protected abbrev FrameClass.trans_wcwf : FrameClass := { F | Reflexive F.Rel ∧ Transitive F.Rel ∧ WeaklyConverseWellFounded F.Rel }
-protected abbrev FrameClass.finite_strict_preorder: FrameClass := { F | F.IsFinite ∧ Reflexive F.Rel ∧ Transitive F.Rel ∧ AntiSymmetric F.Rel }
+protected abbrev FrameClass.finite_partial_order: FrameClass := { F | F.IsFinite ∧ Reflexive F.Rel ∧ Transitive F.Rel ∧ AntiSymmetric F.Rel }
 
 namespace FrameClass.finite_strict_preorder
 
 @[simp]
-lemma nonempty : FrameClass.finite_strict_preorder.Nonempty := by
+lemma nonempty : FrameClass.finite_partial_order.Nonempty := by
   use whitepoint;
   simp [Reflexive , Transitive, AntiSymmetric];
   infer_instance;
 
-lemma validates_AxiomGrz : FrameClass.finite_strict_preorder.ValidatesFormula (Axioms.Grz (.atom 0)) := by
+lemma validates_AxiomGrz : FrameClass.finite_partial_order.ValidatesFormula (Axioms.Grz (.atom 0)) := by
   simp [Validates];
   intro F;
   apply validate_AxiomGrz_of_finite_strict_preorder;
 
-lemma validates_HilbertGrz : Kripke.FrameClass.finite_strict_preorder.Validates Hilbert.Grz.axioms := by
+lemma validates_HilbertGrz : FrameClass.finite_partial_order.Validates Hilbert.Grz.axioms := by
   apply FrameClass.Validates.withAxiomK;
   apply validates_AxiomGrz;
 
@@ -37,11 +37,11 @@ end Kripke
 
 namespace Hilbert.Grz
 
-instance Kripke.finite_sound : Sound (Hilbert.Grz) FrameClass.finite_strict_preorder :=
+instance Kripke.finite_sound : Sound (Hilbert.Grz) FrameClass.finite_partial_order :=
   instSound_of_validates_axioms FrameClass.finite_strict_preorder.validates_HilbertGrz
 
 instance Kripke.consistent : Entailment.Consistent (Hilbert.Grz) :=
-  consistent_of_sound_frameclass FrameClass.finite_strict_preorder (by simp)
+  consistent_of_sound_frameclass FrameClass.finite_partial_order (by simp)
 
 end Hilbert.Grz
 
