Foundation/Modal/Logic/WellKnown.lean
@@ -19,6 +19,8 @@ import Foundation.Modal.Kripke.Hilbert.KTB
 import Foundation.Modal.Kripke.Hilbert.S4
 import Foundation.Modal.Kripke.Hilbert.S4Point2
 import Foundation.Modal.Kripke.Hilbert.S4Point3
+import Foundation.Modal.Kripke.Hilbert.GrzPoint2
+import Foundation.Modal.Kripke.Hilbert.GrzPoint3
 import Foundation.Modal.Kripke.Hilbert.S5
 import Foundation.Modal.Kripke.Hilbert.Triv
 import Foundation.Modal.Kripke.Hilbert.Ver
@@ -142,11 +144,17 @@ instance : (Logic.GL).Unnecessitation := inferInstance
 
 protected abbrev KH : Logic := Hilbert.KH.logic
 
-
 protected abbrev Grz : Logic := Hilbert.Grz.logic
-lemma Grz.eq_ReflexiveTransitiveAntiSymmetricFiniteKripkeFrameClass_Logic : Logic.Grz = Kripke.FrameClass.finite_strict_preorder.logic
+lemma Grz.eq_ReflexiveTransitiveAntiSymmetricFiniteKripkeFrameClass_Logic : Logic.Grz = Kripke.FrameClass.finite_partial_order.logic
   := eq_Hilbert_Logic_KripkeFrameClass_Logic
 
+protected abbrev GrzPoint2 : Logic := Hilbert.GrzPoint2.logic
+lemma GrzPoint2.eq_ReflexiveTransitiveAntiSymmetricConfluentFiniteKripkeFrameClass_Logic : Logic.GrzPoint2 = Kripke.FrameClass.finite_confluent_partial_order.logic
+  := eq_Hilbert_Logic_KripkeFrameClass_Logic
+
+protected abbrev GrzPoint3 : Logic := Hilbert.GrzPoint3.logic
+lemma GrzPoint3.eq_ReflexiveTransitiveAntiSymmetricConnectedFiniteKripkeFrameClass_Logic : Logic.GrzPoint3 = Kripke.FrameClass.finite_connected_partial_order.logic
+  := eq_Hilbert_Logic_KripkeFrameClass_Logic
 
 protected abbrev Triv : Logic := Hilbert.Triv.logic
 lemma Triv.eq_EqualityKripkeFrameClass_Logic : Logic.Triv = Kripke.FrameClass.equality.logic := eq_Hilbert_Logic_KripkeFrameClass_Logic
