Foundation/Modal/Kripke/Hilbert/GrzPoint2.lean
@@ -1,0 +1,85 @@
+import Foundation.Modal.Kripke.Hilbert.Grz.Completeness
+import Foundation.Modal.Kripke.Hilbert.S4Point2
+
+namespace LO.Modal
+
+open Entailment
+open Entailment.Context
+open Formula
+open Formula.Kripke
+open Hilbert.Kripke
+open Kripke
+
+namespace Kripke
+
+abbrev FrameClass.finite_confluent_partial_order : FrameClass := { F | F.IsFinite ∧ Reflexive F.Rel ∧ Transitive F.Rel ∧ AntiSymmetric F.Rel ∧ Confluent F.Rel }
+
+namespace FrameClass.finite_confluent_partial_order
+
+@[simp]
+lemma nonempty : FrameClass.finite_confluent_partial_order.Nonempty := by
+  use whitepoint;
+  simp [Reflexive, Transitive, AntiSymmetric, Confluent ];
+  infer_instance;
+
+lemma validates_HilbertGrzPoint2 : FrameClass.finite_confluent_partial_order.Validates Hilbert.GrzPoint2.axioms := by
+  apply FrameClass.Validates.withAxiomK;
+  rintro F ⟨_, _, _, _, _⟩ φ (rfl | rfl);
+  . apply validate_AxiomGrz_of_finite_strict_preorder;
+    . assumption;
+    . assumption;
+    . assumption;
+  . exact validate_AxiomPoint2_of_confluent $ by assumption;
+
+end FrameClass.finite_confluent_partial_order
+
+end Kripke
+
+
+namespace Hilbert.GrzPoint2.Kripke
+
+instance finite_sound : Sound (Hilbert.GrzPoint2) FrameClass.finite_confluent_partial_order :=
+  instSound_of_validates_axioms FrameClass.finite_confluent_partial_order.validates_HilbertGrzPoint2
+
+instance consistent : Entailment.Consistent (Hilbert.GrzPoint2) :=
+  consistent_of_sound_frameclass FrameClass.finite_confluent_partial_order (by simp)
+
+instance finite_complete : Complete (Hilbert.GrzPoint2) FrameClass.finite_confluent_partial_order :=
+  Kripke.Grz.complete_of_mem_miniCanonicalFrame FrameClass.finite_confluent_partial_order $ by
+    sorry
+    /-
+    intro φ;
+    refine ⟨miniCanonicalFrame.reflexive, miniCanonicalFrame.transitive, miniCanonicalFrame.antisymm, ?_⟩;
+    intro X Y Z ⟨⟨RXY₁, RXY₂⟩, ⟨RXZ₁, RXZ₂⟩⟩;
+    obtain ⟨U, hU⟩ := ComplementClosedConsistentFinset.lindenbaum (𝓢 := Hilbert.GrzPoint2) (Φ := Y.1 ∪ Z.1) (Ψ := φ.subformulasGrz)
+      (by
+        apply Finset.union_subset_iff.mpr;
+        constructor;
+        . intro ψ hψ; exact Y.2.2 |>.subset hψ;
+        . intro ψ hψ; exact Z.2.2 |>.subset hψ;
+      )
+      (by
+        simp [FormulaFinset.Consistent];
+        sorry;
+      );
+    use U;
+    constructor;
+    . constructor;
+      . intro ψ _ hψY; exact hU $ Finset.mem_union.mpr (by tauto);
+      . intro h;
+        ext ξ;
+        constructor;
+        . intro hξY; exact hU $ Finset.mem_union.mpr (by tauto);
+        . sorry;
+    . constructor;
+      . intro ψ _ hψZ; exact hU $ Finset.mem_union.mpr (by tauto);
+      . intro h;
+        ext ξ;
+        constructor;
+        . intro hξZ; exact hU $ Finset.mem_union.mpr (by tauto);
+        . sorry;
+    -/
+
+end Hilbert.GrzPoint2.Kripke
+
+end LO.Modal
