Foundation/Modal/Kripke/Hilbert/GrzPoint3.lean
@@ -1,0 +1,89 @@
+import Foundation.Modal.Kripke.Hilbert.Grz.Completeness
+import Foundation.Modal.Kripke.Hilbert.S4Point3
+
+namespace LO.Modal
+
+open Formula
+open Formula.Kripke
+open Entailment
+open Entailment.Context
+open Kripke
+
+
+open Entailment
+open Entailment.Context
+open Formula
+open Formula.Kripke
+open Hilbert.Kripke
+open Kripke
+
+namespace Kripke
+
+abbrev FrameClass.finite_connected_partial_order : FrameClass := { F | F.IsFinite ∧ Reflexive F.Rel ∧ Transitive F.Rel ∧ AntiSymmetric F.Rel ∧ Connected F.Rel }
+
+namespace FrameClass.finite_connected_partial_order
+
+@[simp]
+lemma nonempty : FrameClass.finite_connected_partial_order.Nonempty := by
+  use whitepoint;
+  simp [Reflexive, Transitive, AntiSymmetric, Connected];
+  infer_instance;
+
+lemma validates_HilbertGrzPoint3 : FrameClass.finite_connected_partial_order.Validates Hilbert.GrzPoint3.axioms := by
+  apply FrameClass.Validates.withAxiomK;
+  rintro F ⟨_, _, _, _, _⟩ φ (rfl | rfl);
+  . apply validate_AxiomGrz_of_finite_strict_preorder;
+    . assumption;
+    . assumption;
+    . assumption;
+  . exact validate_AxiomPoint3_of_connected $ by assumption;
+
+end FrameClass.finite_connected_partial_order
+
+end Kripke
+
+
+namespace Hilbert.GrzPoint3.Kripke
+
+instance finite_sound : Sound (Hilbert.GrzPoint3) FrameClass.finite_connected_partial_order :=
+  instSound_of_validates_axioms FrameClass.finite_connected_partial_order.validates_HilbertGrzPoint3
+
+instance consistent : Entailment.Consistent (Hilbert.GrzPoint3) :=
+  consistent_of_sound_frameclass FrameClass.finite_connected_partial_order (by simp)
+
+instance finite_complete : Complete (Hilbert.GrzPoint3) (FrameClass.finite_connected_partial_order) :=
+  Kripke.Grz.complete_of_mem_miniCanonicalFrame FrameClass.finite_connected_partial_order $ by
+    sorry;
+    /-
+    intro φ;
+    refine ⟨miniCanonicalFrame.reflexive, miniCanonicalFrame.transitive, miniCanonicalFrame.antisymm, ?_⟩;
+    intro x y z ⟨⟨Rxy₁, Rxy₂⟩, ⟨Rxz₁, Rxz₂⟩⟩;
+    apply or_iff_not_imp_left.mpr;
+    intro nRyz;
+    rcases (not_and_or.mp nRyz) with (nRyz | nRyz);
+    . push_neg at nRyz;
+      obtain ⟨ψ, hψ, ⟨hψy, hψz⟩⟩ := nRyz;
+      constructor;
+      . intro ξ hξ₁ hξ₂;
+        apply Rxy₁;
+        . exact hξ₁;
+        . sorry;
+      . intro hyz;
+        have exy := Rxy₂ ?_;
+        have exz := Rxz₂ ?_;
+        tauto;
+        . subst exy;
+          intro ξ hξ hξz;
+          sorry;
+        . intro ξ hξ hξy;
+          sorry;
+    . push_neg at nRyz;
+      replace ⟨nRyz₁, nRyz₂⟩ := nRyz;
+      constructor;
+      . sorry;
+      . sorry;
+    -/
+
+end Hilbert.GrzPoint3.Kripke
+
+end LO.Modal
